\subsection{Introduction}
\begin{definition}
	If \( f \colon [a,b] \subset \mathbb R \to \mathbb C \) is a complex function, and the real and imaginary parts of \( f \) are Riemann integrable, then we define
	\[ \int_a^b f(t) \dd{t} = \int_a^b \Re(f(t)) \dd{t} + i \int_a^b \Im(f(t)) \dd{t} \]
	In particular, for \( g \colon [a,b] \to \mathbb R \), we have
	\[ \int_a^b ig(t) \dd{t} = i\int_a^b g(t) \dd{t} \]
	Thus, for a complex constant \( w \in \mathbb C \), we can find
	\[ \int_a^b wf(t) \dd{t} = w \int_a^b f(t) \dd{t} \]
\end{definition}
\begin{proposition}[basic estimate]
	If \( f \colon [a,b] \to \mathbb C \) is continuous, then
	\[ \abs{\int_a^b f(t) \dd{t}} \leq \int_a^b \abs{f(t)} \dd{t} \leq (b-a) \sup_{t \in [a,b]} \abs{f(t)} \]
	Equality holds if and only if \( f \) is constant.
\end{proposition}
\begin{proof}
	If \( \int_a^b f(t) \dd{t} = 0 \) then the proof is complete.
	Otherwise, we can write the value of the integral as \( re^{i\theta} \) for \( \theta \in [0, 2\pi) \).
	Let \( M = \sup_{t \in [a,b]} \abs{f(t)} \).
	Then we have
	\begin{align*}
		\abs{\int_a^b f(t) \dd{t}} &= r \\
		&= e^{-i\theta} \int_a^b f(t) \dd{t} \\
		&= \int_a^b e^{-i\theta} f(t) \dd{t} \\
		&= \int_a^b \Re(e^{-i\theta} f(t)) \dd{t} + i \int_a^b \Im(e^{-\theta f(t)}) \dd{t}
	\end{align*}
	Since the left hand side is real, the imaginary integral vanishes.
	\begin{align*}
		\abs{\int_a^b f(t) \dd{t}} &= \int_a^b \Re(e^{-i\theta} f(t)) \dd{t} \\
		&\leq \int_a^b \abs{e^{-i\theta} f(t)} \dd{t} = \int_a^b \abs{f(t)} \dd{t} \\
		&\leq (b-a)M
	\end{align*}
	Equality holds if and only if \( \abs{f(t)} = M \) and \( \Re(e^{-i\theta} f(t)) = M \) for all \( t \in [a,b] \), which is true only if \( \abs{f(t)} = M \) and \( \arg(f(t)) = \theta \) hence \( f = Me^{i\theta} \) for all \( t \).
\end{proof}

\subsection{Integrating along curves}
\begin{definition}
	Let \( U \subset \mathbb C \) be an open set and let \( f \colon U \to \mathbb C \) be continuous.
	Let \( \gamma \colon [a,b] \to U \) be a \( C^1 \) curve.
	Then the \textit{integral of \( f \) along \( \gamma \)} is
	\[ \int_\gamma f(z) \dd{z} = \int_a^b f(\gamma(t)) \gamma'(t) \dd{t} \]
\end{definition}
This definition is consistent with the previous definition of the integral of a function \( f \) along the interval \( [a,b] \).
The integral along a curve has various convenient properties.
\begin{enumerate}[(i)]
	\item It is invariant under the choice of parametrisation.
		Let \( \varphi \colon [a_1, b_1] \to [a,b] \) be \( C^1 \) and injective with \( \varphi(a_1) = a \) and \( \varphi(b_1) = b \).
		Let \( \delta = \gamma \circ \varphi \colon [a_1, b_1] \to U \).
		Then
		\[ \int_\delta f(z) \dd{z} = \int_\gamma f(z) \dd{z} \]
		Indeed,
		\begin{align*}
			\int_\delta f(z) \dd{z} &= \int_{a_1}^{b_1} f(\gamma (\varphi(t))) \gamma'(\varphi(t)) \varphi'(t) \dd{t} \\
			&= \int_a^b f(\gamma(s)) \gamma'(s) \dd{s} \\
			&= \int_\gamma f(z) \dd{z}
		\end{align*}
	\item The integral is linear.
		It is easy to check that
		\[ \int_\gamma (\lambda f(z) + \mu g(z)) \dd{z} = \lambda \int_\gamma f(z) \dd{z} + \mu \int_\gamma g(z) \dd{z} \]
		for complex constants \( \lambda, \mu \in \mathbb C \).
	\item The additivity property states that if \( \gamma \colon[a,b] \to U \) is \( C^1 \) and \( a < c < b \), then
		\[ \int_\gamma f(z) \dd{z} = \int_{\eval{\gamma}_{[a,c]}} f(z) \dd{z} + \int_{\eval{\gamma}_{c,b}} f(z) \dd{z} \]
	\item We define the \textit{inverse path} \( (-\gamma) \colon [-b, -a] \to U \) by \( (-\gamma)(t) = \gamma(-t) \).
		Then
		\[ \int_{(-\gamma)} f(z) \dd{z} = \int_\gamma f(z) \dd{z} \]
\end{enumerate}
\begin{definition}
	Let \( \gamma \colon [a,b] \to \mathbb C \) be a \( C^1 \) curve.
	Then the \textit{length} of \( \gamma \) is
	\[ \mathrm{length}(\gamma) = \int_a^b \abs{\gamma'(t)} \dd{t} \]
\end{definition}
\begin{definition}
	A \textit{piecewise \( C^1 \) curve} is a continuous map \( \gamma \colon [a,b] \to \mathbb C \) such that there exists a finite subdivision
	\[ a < a_0 < a_1 < \dots < a_n = b \]
	such that each \( \gamma_j = \eval{\gamma}_{[a_{j-1}, a_j]} \) is \( C^1 \) for \( 1 \leq j \leq n \).
	Then, for such a piecewise \( C^1 \) curve, we define
	\[ \int_\gamma f(z) \dd{z} = \sum{j=1}^n \int_{\gamma_j} f(z) \dd{z} \]
	and
	\[ \mathrm{length}(\gamma) = \sum_{j=1}^n \mathrm{length}(\gamma_j) = \sum_{j=1}^n \int_{a_{j-1}}^{a_j} \abs{\gamma'(t)} \dd{t} \]
	By the additivity property, both definitions are invariant under changing the subdivision.
	From here, we will use `curve' to refer to `piecewise \( C^1 \) curve', unless stated otherwise.
\end{definition}
\begin{definition}
	If \( \gamma_1 \colon [a,b] \to \mathbb C \) and \( \gamma_2 \colon [c,d] \) are curves with \( \gamma_1(b) = \gamma_2(c) \), we define the \textit{sum} of \( \gamma_1 \) and \( \gamma_2 \) to be the curve
	\[ (\gamma_1 + \gamma_2) \colon [a,b+d-c] \to \mathbb C;\quad (\gamma_1 + \gamma_2)(t) = \begin{cases}
		\gamma_1(t) & a \leq t \leq b \\
		\gamma_2(t - b + c) & b \leq t \leq b + d - c
	\end{cases} \]
\end{definition}
\begin{proposition}
	Let \( f \colon U \to \mathbb C \) be continuous and \( \gamma \colon [a,b] \to \mathbb C \), we have
	\[ \abs{\int_\gamma f(z) \dd{z}} \leq \mathrm{length}(\gamma) \sup_\gamma \abs{f} \]
	where \( \sup_\gamma g \equiv \sup_{t \in [a,b]} g(\gamma(t)) \).
\end{proposition}
\begin{proof}
	If \( \gamma \) is \( C^1 \), then
	\[ \abs{\int_\gamma f(z) \dd{z}} = \abs{\int_a^b f(\gamma(t)) \gamma'(t) \dd{t}} \leq \int_a^b \abs{f(\gamma(t))} \cdot \abs{\gamma'(t)} \dd{t} \leq \sup_{t \in [a,b]} \abs{f(\gamma(t))} \mathrm{length}(\gamma) \]
	If \( \gamma \) is piecewise \( C^1 \), then the result follows from the definition of a piecewise \( C^1 \) function and the above.
\end{proof}

\subsection{Fundamental theorem of calculus}
\begin{theorem}[fundamental theorem of calculus]
	Let \( f \colon U \to \mathbb C \) be continuous on an open set \( U \subset \mathbb C \).
	Let \( F \colon U \to \mathbb C \) be a function such that \( F'(z) = f(z) \) for all \( z \in U \).
	Then, for any curve \( \gamma \colon [a,b] \to U \), we have
	\[ \int_\gamma f(z) \dd{z} = F(\gamma(b)) - F(\gamma(a)) \]
	If \( \gamma \) is a closed curve, then \( \int_\gamma f(z) = 0 \).
	Such a function \( F \) is known as an \textit{antiderivative} of \( f \).
\end{theorem}
\begin{proof}
	\[ \int_\gamma f(z) \dd{z} = \int_a^b f(\gamma(t)) \gamma'(t) \dd{t} = \int_a^b \dv{t} F(\gamma(t)) \dd{t} = F(\gamma(b)) - F(\gamma(a)) \]
\end{proof}
\begin{remark}
	Note that we assume that \( f \) exists such that \( F'(z) = f(z) \); such an \( f \) is not provided for by the theorem.
	A function \( F \) satisfying these criteria is called an \textit{antiderivative} of \( f \).
\end{remark}
\begin{example}
	For an integer \( n \) and the curve \( \gamma(t) = Re^{2\pi it} \) for \( t = [0,1] \), consider the integral \( \int_\gamma z^n \dd{z} \).
	For \( n \neq -1 \), the function \( \frac{z^{n+1}}{n+1} \) is an antiderivative of \( z^n \).
	Hence, \( \int_\gamma z^n \dd{z} = 0 \) since \( \gamma \) is a closed curve.
	If \( n = -1 \), we can use the definition of the integral to find
	\[ \int_\gamma \frac{1}{z} \dd{z} = \int_0^1 \frac{1}{\gamma(t)} \gamma'(t) \dd{t} = \int_0^1 \frac{1}{Re^{2\pi i t}}2\pi i R e^{2 \pi i t} \dd{t} = 2 \pi i \]
	This is not zero, hence for all \( R > 0 \), \( \frac{1}{z} \) has no antiderivative in any open set containing the circle \( \qty{\abs{z} = R} \).
	In particular, for any branch of logarithm \( \lambda \), it has derivative \( \frac{1}{z} \), hence there exists no branch of logarithm on \( \mathbb C^\star = \mathbb C \setminus \qty{0} \).
\end{example}
\begin{theorem}[converse to fundamental theorem of calculus]
	Let \( U \subset \mathbb C \) be a domain.
	If \( f \colon U \to \mathbb C \) is continuous and if \( \int_\gamma f(z) \dd{z} = 0 \) for every closed curve \( \gamma \) in \( U \), then \( f \) has an antiderivative.
	In other words, there exists a holomorphic function \( F \colon U \to \mathbb C \) such that \( F' = f \) in \( U \).
\end{theorem}
\begin{proof}
	Let \( a_0 \in U \).
	Then for \( w \in U \), we can define
	\[ F(w) = \int_{\gamma_w} f(z) \dd{z} \]
	where \( \gamma_w \colon [0,1] \to \mathbb C \) is a curve with \( \gamma_w(0) = a_0 \) and \( \gamma_w(1) = w \).

	The definition of \( F \) is independent of the choice of \( \gamma_w \) is independent of the choice of \( \gamma_w \).
	Indeed, suppose two paths \( \gamma_w, \gamma_w' \) exist.
	Then the curve \( \gamma_w + (-\gamma_w') \) is a closed path, and by assumption the integral along this curve is zero.
	Thus \( F \) is independent of the choice of path as claimed.
	So \( F \) is a well-defined function.

	Now, let \( w \in U \).
	Since \( U \) is an open set, there exists \( r > 0 \) such that \( D(w,r) \subset U \).
	For \( h \in \mathbb C \) with \( 0 < \abs{h} < r \), let \( \delta_h \) be the radial path \( t \mapsto w + th \) for \( t \in [0,1] \).
	Now we define
	\[ \gamma = \gamma_w + \delta_h + (-\gamma_{w+h}) \]
	This is a closed curve contained within \( U \), hence \( \int_\gamma f(z) \dd{z} = 0 \).
	Thus
	\[ \int_{\gamma_{w+h}} f(z) \dd{z} = \int_{\gamma_w} f(z) \dd{z} + \int_{\delta_h} f(z) \dd{z} \]
	Informally, the integral has an additivity property which is independent of the path taken.
	Rewriting this using \( F \),
	\begin{align*}
		F(w+h) &= F(w) + \int_{\delta_h} f(z) \dd{z} \\
		&= F(w) + \int_{\delta_h} (f(z) + f(w) - f(w)) \dd{z} \\
		&= F(w) + hf(w) + \int_{\delta_h} (f(z) - f(w)) \dd{z}
	\end{align*}
	Hence, by continuity of \( f \),
	\begin{align*}
		\abs{\frac{F(w+h) - F(w)}{h} - f(w)} &= \frac{1}{\abs{h}} \abs{\int_{\delta_h} (f(z) - f(w)) \dd{z}} \\
		&\leq \frac{1}{\abs{h}} \mathrm{length}(\delta_h) \sup_{z \in \Im \delta_h} \abs{f(z) - f(w)} \\
		&= \sup_{z \in \Im \delta_h} \abs{f(z) - f(w)} \\
		\therefore \lim_{h \to 0} \abs{\frac{F(w+h) - F(w)}{h} - f(w)} &= \lim_{h \to 0} \sup_{z \in \Im \delta_h} \abs{f(z) - f(w)} = 0
	\end{align*}
	Thus, \( F \) is differentiable at \( w \) with \( F'(w) = f(w) \).
\end{proof}

\subsection{Star-shaped domains}
\begin{definition}
	A domain \( U \) is \textit{star-shaped}, or a \textit{star domain}, if there exists a (not necessarily unique) centre \( a_0 \in U \) such that for all \( w \in U \), the straight line segment \( [a_0, w] \) is contained within \( U \).
\end{definition}
\begin{remark}
	Any disk is convex; any convex domain is star-shaped; any star-shaped domain is path-connected.
	The reverse implications are not true in general.
\end{remark}
\begin{definition}
	A \textit{triangle} in \( \mathbb C \) is the \textit{convex hull} of three points in \( \mathbb C \).
	The (closed) convex hull of a set \( S \) is the smallest (closed) convex set \( C \) such that \( S \subseteq C \).
	In this case, if \( z_1, z_2, z_3 \in \mathbb C \), we have
	\[ T = \qty{az_1 + bz_2 + cz_3 \colon 0 \leq a,b,c \leq 1, a+b+c=1} \]
	When used as a curve, the boundary \( \partial T \) represents the piecewise affine closed curve \( \gamma = \gamma_1 + \gamma_2 + \gamma_3 \) where \( \gamma_i \) are affine functions parametrising the three line segments on the boundary of \( T \).
\end{definition}
\begin{corollary}
	Let \( U \) be a star-shaped domain.
	Let \( f \colon U \to \mathbb C \) be continuous and \( \int_{\partial T} f(z) \dd{z} = 0 \) for any triangle \( T \subset U \).
	Then \( f \) has an antiderivative in \( U \).
\end{corollary}
\begin{remark}
	This is a relaxation of the conditions from the previous theorem.
\end{remark}
\begin{proof}
	Let \( a_0 \) be a centre for the domain \( U \).
	Let \( w \) be an arbitrary point in \( U \).
	Then let \( \gamma_w \) be the affine function parametrising the directed line segment \( [a_0,w] \), and let \( F(w) = \int_{\gamma_w} f(z) \dd{z} \).
	Using \( h \) and \( \delta_h \) as above, by letting \( \gamma = \gamma_w + \delta_h + (-\gamma_{w+h}) \) we then have \( \int f(z) \dd{z} = \pm \int_{\partial T} f(z) \dd{z} \) for a triangle \( T \subset U \).
	Since the integral around a triangle is zero by hypothesis, \( \int_\gamma f(z) \dd{z} = 0 \).
	We then complete the proof in analogous way to the general case.
\end{proof}
\begin{theorem}[Cauchy's theorem for triangles]
	Let \( U \subset \mathbb C \) be an open set and \( f \colon U \to \mathbb C \) be a holomorphic function.
	Then \( \int_{\partial T} f(z) \dd{z} = 0 \) for all triangles \( T \subset U \).
\end{theorem}
\begin{proof}
	Let \( \eta(t) = \int_{\partial T} f(z) \dd{z} \).
	We will subdivide the triangle \( T \) into four smaller triangles \( T^{(1)}, T^{(2)}, T^{(3)}, T^{(4)} \).
	The vertices of the inner triangle are the midpoints of the sides of \( T \), and the three other triangles are constructed to fill the remaining area of \( T \).
	Thus,
	\[ \eta(T) = \int_{\partial T^{(1)}} f(z) \dd{z} + \int_{\partial T^{(2)}} f(z) \dd{z} + \int_{\partial T^{(3)}} f(z) \dd{z} + \int_{\partial T^{(4)}} f(z) \dd{z} \]
	Then, by the triangle inequality, there exists a triangle \( T^{(j)} \) such that
	\[ \abs{\int_{\partial T^{(j)}} f(z) \dd{z}} \geq \frac{\abs{\eta(T)}}{4} \]
	Let \( T_0 = T \), and \( T_1 = T^{(j)} \), so \( \abs{\eta(T_1)} \geq \frac{1}{4}\abs{\eta(T_0)} \).
	We can show geometrically that for any choice of \( T_i \), \( \mathrm{length}(\partial T_1) = \frac{1}{2}\mathrm{length}(\partial T_0) \).
	Inductively, we can subdivide \( T_i \) and produce \( T_{i+1} \), such that
	\[ T_0 \supset T_1 \supset \cdots;\quad \abs{\eta(T_n)} \geq \frac{1}{4}\abs{\eta(T_{n-1})};\quad \mathrm{length}(\partial T_n) = \frac{1}{2} \mathrm{length}(\partial T_{n-1}) \]
	Hence,
	\[ \abs{\eta(T_n)} \geq \frac{1}{4^n}\abs{\eta(T_0)};\quad \mathrm{length}(\partial T_n) = \frac{1}{2^n} \mathrm{length}(\partial T_0) \]
	Since \( T_n \) are non-empty, nested closed subsets with diameter converging to zero, we can show that \( \bigcap_{n=1}^\infty T_n = \qty{z_0} \) for some \( z_0 \in \mathbb C \).
	Let \( \varepsilon > 0 \).
	Since \( f \) is differentiable at \( z_0 \), there exists \( \delta > 0 \) such that
	\begin{align*}
		z \in U, \abs{z - z_0} < \delta &\implies \abs{\frac{f(z) - f(z_0)}{z - z_0} - f'(z_0)} \leq \varepsilon \\
		&\implies \abs{f(z) - f(z_0) - f'(z_0)(z - z_0)} \leq \varepsilon \abs{z - z_0}
	\end{align*}
	Now, observe that for all \( n \),
	\[ \int_{\partial T_n} f(z) \dd{z} = \int_{\partial T_n} (f(z) - f(z_0) - f'(z_0)(z - z_0)) \dd{z} \]
	since \( \int_{\partial T_n} \dd{z} = \int_{\partial T_n} z \dd{z} = 0 \) by the fundamental theorem of calculus.
	Let \( n \) such that \( T_n \subset D(z_0, \delta) \).
	Hence,
	\begin{align*}
		\frac{1}{4^n} \abs{\eta(T_0)} &\leq \abs{\eta(T_n)} \\
		&= \abs{\int_{\partial T_n} f(z) \dd{z}} \\
		&= \abs{\int_{\partial T_n} (f(z) - f(z_0) - f'(z_0)(z - z_0)) \dd{z}} \\
		&\leq \qty(\sup_{z \in \partial T_n} \abs{f(z) - f(z_0) - f'(z_0)(z-z_0)}) \mathrm{length}(\partial T_n) \\
		&\leq \varepsilon \qty(\sup_{z \in \partial T_n} \abs{z - z_0}) \mathrm{length}(\partial T_n) \\
		&\leq \varepsilon \mathrm{length}(\partial T_n)^2 \\
		&= \frac{\varepsilon}{4^n} \mathrm{length}(\partial T_0)^2 \\
		\therefore \abs{\eta(T_0)} &\leq \varepsilon \mathrm{length}(\partial T_0)^2
	\end{align*}
	\( \varepsilon \) was arbitrary, hence \( \eta(T_0) \) must be zero.
\end{proof}
We can generalise the above theorem for functions that are holomorphic except at a finite number of points.
\begin{theorem}
	Let \( U \subset \mathbb C \) be an open set and \( f \colon U to \mathbb C \) be a continuous function.
	Let \( S \subset U \) be a finite set and suppose that \( f \) is holomorphic on \( U \setminus S \).
	Then \( \int_{\partial T} f(z) \dd{z} = 0 \) for all triangles \( T \subset U \).
\end{theorem}
\begin{proof}
	By the procedure above, we can subdivide \( T \) into a total of \( 4^n \) smaller triangles; at each step we join the midpoints of the sides of the triangles of the previous step.
	We will keep all of the smaller triangles, and let the sequence of such smaller triangles be denoted \( T_1, \dots, T_N \).
	Then, since the integrals along the sides of the smaller triangles that are interior to \( T \) cancel, we have
	\[ \int_{\partial T} f(z) \dd{z} = \sum_{j=1}^N \int_{\partial T_j} f(z) \dd{z} \]
	By the previous theorem, \( \int_{\partial T_j} f(z) \dd{z} = 0 \) unless \( T_j \) intersects with \( S \).
	So by letting \( I = \qty{j \colon T_j \cap S \neq \varnothing} \), we have
	\[ \int_{\partial T} f(z) \dd{z} = \sum_{j \in I} \int_{\partial T_j} f(z) \dd{z} \]
	Since any point may be in at most six of the smaller triangles, and \( \mathrm{length}(\partial T_j) = \frac{1}{2^n} \mathrm{length}(\partial T) \), we find
	\[ \abs{\int_{\partial T} f(z) \dd{z}} \leq 6\abs{S} \qty(\sup_{z \in T} \abs{f(z)}) \frac{\mathrm{length}(\partial T)}{2^n} \]
	Then let \( n \to \infty \) and the result then holds as rqeuired.
\end{proof}
We can now prove the `convex Cauchy' theorem.
\begin{corollary}[Cauchy's theorem for convex sets]
	Let \( U \subset \mathbb C \) be convex, or more generally, a star domain.
	Let \( f \colon U \to \mathbb C \) be continuous, and holomorphic in \( U \setminus S \) where \( S \) is a finite set.
	Then \( \int_\gamma f(z) \dd{z} = 0 \) for any closed curve \( \gamma \) in \( U \).
\end{corollary}
\begin{proof}
	By the theorems above, \( \int_{\partial T} f(z) \dd{z} = 0 \) for any triangle \( T \subset U \).
	Since \( U \) is a star domain and \( f \) is continuous, this means that \( f \) has an antiderivative in \( U \).
	The result then follows from the fundamental theorem of calculus.
\end{proof}
\begin{remark}
	We will soon show that if \( f \colon U \to \mathbb C \) is continuous and holomorphic in \( U \setminus S \) where \( S \) is finite, then \( f \) is holomorphic in \( U \).
\end{remark}

\subsection{Cauchy's integral formula}
For a disk \( D(a,\rho) \) we will write \( \int_{\partial D(a,\rho)} f(z) \dd{z} \) to mean \( \int_\gamma f(z) \dd{z} \) where \( \gamma \colon [0,1] \to \mathbb C \) is the curve \( \gamma(t) = a+\rhoe^{2\pi i t} \).
\begin{theorem}[Cauchy's integral formula for a disk]
	Let \( D = D(a,r) \) and let \( f \colon D \to \mathbb C \) be holomorphic.
	Then, for any \( \rho \) with \( 0 < \rho < r \) and any \( w \in D(a,\rho) \), we have
	\[ f(w) = \frac{1}{2\pi i} \int_{\partial D(a,\rho)} \frac{f(z) \dd{z}}{z-w} \]
	In particular, taking \( w = a \),
	\[ f(a) = \frac{1}{2\pi i} \int_{\partial D(a,\rho)} \frac{f(z) \dd{z}}{z-a} = \int_0^1 f(a+\rho e^{2\pi i t}) \dd{t} \]
	This final equation is called the \textit{mean value property} for holomorphic functions.
\end{theorem}
We first need the following lemma.
\begin{lemma}
	If \( \gamma \colon [a,b] \to \mathbb C \) is a curve and \( (f_n) \) is a sequence of continuous complex functions on \( \Im \gamma \) converging uniformly to \( f \) on \( \Im\gamma \), then \( \int_\gamma f_n(z) \dd{z} \to \int_\gamma f(z) \dd{z} \).
\end{lemma}
\begin{proof}
	We have
	\[ \abs{\int_\gamma f_n(z) \dd{z} - \int_\gamma f(z) \dd{z}} = \abs{\int_\gamma (f_n(z) - f(z)) \dd{z}} \leq \sup_{z \in \Im \gamma} \abs{f_n(z) - f(z)} \mathrm{length}(\gamma) \]
\end{proof}
We can now prove Cauchy's integral formula for a disk.
\begin{proof}
	Let \( w \in D(a,\rho) \) be fixed, and define \( h \colon D \to \mathbb C \) by
	\[ h(z) = \begin{cases}
		\frac{f(z) - f(w)}{z - w} & \text{if } z \neq w \\
		f'(w) & \text{if } z = w
	\end{cases} \]
	Then \( h \) is continuous on \( D \) and holomorphic in \( D \setminus \qty{w} \).
	By Cauchy's theorem for convex sets,
	\[ \int_{\partial D(a,\rho)} h(z) \dd{z} = 0 \]
	Substituting for \( h \), we find
	\[ f(w) \int_{\partial D(a,\rho)} \frac{\dd{z}}{z-w} = \int_{\partial D(a,\rho)} \frac{f(z) \dd{z}}{z-w} \]
	It now suffices to prove that
	\[ \int_{\partial D(a,\rho)} \frac{\dd{z}}{z-w} = 2 \pi i \]
	Note that
	\[ \frac{1}{z-w} = \frac{1}{z-a+a-w} = \frac{1}{\qty(z-a)\qty(1 - \frac{w-a}{z-a})} = \sum_{j=0}^\infty \frac{(w-a)^j}{(z-a)^{j+1}} \]
	where the convergence is uniform for \( z \in \partial D(a,\rho) \) by the Weierstrass \( M \)-test.
	Therefore, by the above lemma, we interchange summation and integration to find
	\[ \int_{\partial D(a,\rho)} \frac{\dd{z}}{z-w} = \sum_{j=0}^\infty (w-a)^j \int_{\partial D(a,\rho)} \frac{\dd{z}}{(z-a)^{j+1}} \]
	For \( j \geq 1 \), the function \( \frac{1}{(z-a)^{j+1}} \) has an antiderivative in a neighbourhood of \( \partial D(a,\rho) \), hence all integrals on the right hand side for \( j \geq 1 \) vanish.
	For \( j = 0 \), we can compute directly that \( \int_{\partial D(a,\rho)} \frac{\dd{z}}{z-a} = 2 \pi i \).
	Hence, \( \int_{\partial D(a,\rho)} \frac{\dd{z}}{z-w} = 2 \pi i \), proving Cauchy's intgeral formula.

	Now, taking \( w = a \) in Cauchy's integral formula, we find
	\[ f(a) = \frac{1}{2\pi i} \int_{\partial D(a,\rho)} \frac{f(z) \dd{z}}{z-a} \]
	By direct computation using the parametrisation \( t \mapsto a + \rho e^{2\pi i t} \) for \( t \in [0,1] \), we find
	\[ f(a) = \int_0^1 f(a+\rho e^{2 \pi i t}) \dd{t} \]
	as required.
\end{proof}

\subsection{Liouville's theorem}
\begin{theorem}
	Let \( f \colon \mathbb C \to \mathbb C \) be entire and bounded.
	Then \( f \) is constant.
	More generally, if \( f \) is entire with sublinear growth (there exist \( K \geq 0 \) and \( \alpha < 1 \) such that \( \abs{f(z)} \leq K(1+\abs{z}^\alpha) \) for all \( z \in \mathbb C \)) then \( f \) is constant.
\end{theorem}
\begin{proof}
	Let \( w \in \mathbb C \) and \( \rho > \abs{w} \).
	By Cauchy's integral formula, we have
	\[ f(w) = \frac{1}{2 \pi i} \int_{\partial D(0,\rho)} \frac{f(z)\dd{z}}{z-w};\quad f(0) = \frac{1}{2 \pi i} \int_{\partial D(0,\rho)} \frac{f(z) \dd{z}}{z} \]
	Thus,
	\begin{align*}
		\abs{f(w) - f(0)} &= \frac{1}{2\pi} \abs{\int_{\partial D(0,\rho)} \frac{wf(z) \dd{z}}{z(z-w)}} \\
		&\leq \frac{\abs{w}}{2 \pi} \sup_{z \in \partial D(0,\rho)} \frac{\abs{f(z)}}{\abs{z} \cdot \abs{\abs{z} - \abs{w}}} \mathrm{length}(\partial D(0,\rho)) \\
		&\leq \frac{\abs{w} K(1+\rho^\alpha)}{2\pi \rho(\rho - \abs{w})} 2 \pi \rho \\
		&= \frac{\abs{w}K(1+\rho^\alpha)}{\rho - \abs{w}}
	\end{align*}
	By letting \( \rho \to \infty \), we can conclude \( f(w) = f(0 )\).
\end{proof}
\begin{theorem}[fundamental theorem of algebra]
	Every non-constant polynomial with complex coefficients has a complex root.
\end{theorem}
\begin{proof}
	Let \( p(z) = a_n z^n + \dots + a_0 \) be a complex polynomial of degree \( n \geq 1 \).
	Then \( a_n \neq 0 \), and for \( z \neq 0 \) we can write
	\[ p(z) = z^n \qty(a_n + \frac{a_{n-1}}{z} + \dots + \frac{a_0}{z^n} ) \]
	By the triangle inequality,
	\[ \abs{p(z)} \geq \abs{z}^n \qty(\abs{a_n} - \frac{\abs{a_{n-1}}}{\abs{z}} - \dots - \frac{\abs{a_0}}{\abs{z}^n} \]
	Hence, there exists \( R > 0 \) such that \( \abs{p(z)} \geq 1 \) for \( \abs{z} > R \).

	Now, if \( p(z) \neq 0 \) for all \( z \), then \( g(z) = \frac{1}{p(z)} \) is entire.
	By the above, \( \abs{g(z)} \leq 1 \) for \( \abs{z} > R \).
	By continuity of \( g \), we have further that \( \abs{g(z)} \) is bounded from above on the compact set \( \qty{\abs{z} \leq R} \).
	Hence, \( g \) is a bounded entire function.
	By Liouville's theorem, \( g \) is constant.
	Since \( p \) is non-constant, this is a contradiction.
	Hence \( p \) has a zero.
\end{proof}
\begin{theorem}[local maximum modulus principle]
	Let \( f \colon D(a,R) \to \mathbb C \) be holomorphic, and \( \abs{f(z)} \leq \abs{f(a)} \) for all \( z \in D(a,R) \).
	Then \( f \) is constant.
\end{theorem}
\begin{proof}
	By the mean value property,
	\[ f(a) = \int_0^1 f(a+\rho e^{2 \pi i t}) \dd{t} \]
	Therefore,
	\[ \abs{f(a)} = \abs{\int_0^1 f(a + \rho e^{2 \pi i t}) \dd{t}} \leq \sup_{t \in [0,1]} \abs{f(a+\rho e^{2 \pi i t})} \leq \abs{f(a)} \]
	where the last inequality is by hypothesis.
	Therefore, both inequalities must be equalities.
	Equality in the first inequality implies that \( f(a+\rho e^{2 \pi i t}) = c_\rho \) for some constant \( c_\rho \) and all \( t \in [0,1] \).
	Then, by the first equality, \( \abs{c_\rho} = \abs{f(a)} \) for all \( \rho \in (0,R) \).
	Thus, \( \abs{f(a+\rho e^{2 \pi i t})} \) is constant for all \( \rho \in (0,R) \) and \( t \in [0,1] \).
	Hence \( \abs{f(z)} \) is constant on \( D(a,R) \).
	By the Cauchy-Riemann equations, \( f \) must be constant.
\end{proof}

\subsection{Taylor series}
\begin{theorem}

\end{theorem}
