\subsection{Stirling's Formula}
Let $(a_n)$ and $(b_n)$ be sequences. We will write $a_n \sim b_n$ if $\frac{a_n}{b_n} \to 1$ as $n \to \infty$. This is asymptotic equality.
\begin{theorem}[Stirling's Formula]
	$n! \sim n^n\, \sqrt{2 \pi n}\, e^{-n}$ as $n \to \infty$.
\end{theorem}
\noindent Let us first prove the weaker statement $\log (n!) \sim n \log n$.
\begin{proof}
	Let us define $l_n = \log (n!) = \log 2 + \log 3 + \dots + \log n$. For $x \in \mathbb R$, we write $\floor{x}$ for the integer part of $x$. Note that
	\[ \log \floor x \leq \log x \leq \log \floor{x+1} \]
	Let us integrate this from 1 to $n$.
	\[ \sum_{k=1}^{n-1} \log k \leq \int_1^n \log x\, \dd{x} \leq \sum_{k=2}^{n} \log k \]
	\[ l_{n-1} \leq n \log n - n + 1 \leq l_n \]
	For all $n$, therefore:
	\[ n \log n - n + 1 \leq l_n \leq (n+1) \log (n+1) - (n+1) + 1 \]
	Dividing through by $n\log n$, we get
	\[ \frac{l_n}{n \log n} \to 1 \]
	as $n \to \infty$.
\end{proof}
\noindent The following complete proof is non-examinable.
\begin{proof}
	For any twice-differentiable function $f$, for any $a < b$ we have
	\[ \int_a^b f(x) \dd{x} = \frac{f(a) + f(b)}{2} (b - a) - \frac{1}{2}\int_a^b (x-a)(b-x)f''(x)\dd{x} \]
	Now let $f(x) = \log x$, $a=k$ and $b=k+1$. Then
	\begin{align*}
		\int_k^{k+1} \log x \dd{x} & = \frac{\log k + \log(k+1)}{2} + \frac{1}{2}\int_k^{k+1} \frac{(x-k)(k+1-x)}{x^2}\dd{x}                            \\
		                           & = \frac{\log k + \log(k+1)}{2} + \frac{1}{2}\int_0^1 \frac{x(1-x)}{(x+k)^2}\dd{x}                                  \\
		\intertext{Let us take the sum for $k=1, \dots, n-1$ of the equality.}
		\int_1^n \log x \dd{x}     & = \frac{\log ((n-1)!) + \log(n!)}{2} + \frac{1}{2}\sum_{k=1}^{n-1}\int_0^1 \frac{x(1-x)}{(x+k)^2}\dd{x}            \\
		n\log n - n + 1            & = \log (n!) - \frac{\log n}{2} + \sum_{k=1}^{n-1} a_k;\quad a_k = \frac{1}{2}\int_0^1 \frac{x(1-x)}{(x+k)^2}\dd{x} \\
		\log (n!)                  & = n \log n - n + \frac{\log n}{2} + 1 - \sum_{k=1}^{n-1} a_k                                                       \\
		n!                         & = n^n \, e^{-n} \, \sqrt n \, \exp\left( 1 - \sum_{k=1}^{n-1} a_k \right)
	\end{align*}
	Now, note that
	\[ a_k \leq \frac{1}{2}\int_0^1 \frac{x(1-x)}{k^2}\dd{x} = \frac{1}{12k^2} \]
	So the sum of all $a_k$ converges. We set
	\[ A = \exp\left( 1 - \sum_{k=1}^\infty a_k \right) \]
	and then
	\[ n! = n^n \, e^{-n} \, \sqrt n \, A \, \exp\left( \underbrace{\sum_{k=n}^\infty a_k}_{\text{converges to zero}} \right) \]
	Therefore,
	\[ n! \sim n^n\, \sqrt{n}\, e^{-n}\, A \]
	To finish the proof, we must show that $A = \sqrt{2 \pi}$. We can utilise the fact that $n! \sim n^n\, \sqrt{n}\, e^{-n}\, A$.
	\begin{align*}
		2^{-2n} \binom{2n}{n} & = 2^{-2n} \cdot \frac{2n!}{(n!)^2}                                                                                           \\
		                      & \sim 2^{-2n} \frac{(2n)^{2n} \cdot \sqrt{2n} \cdot A \cdot e^{-2n}}{n^n\, e^{-n}\, \sqrt n\, A\, n^n\, e^{-n}\, \sqrt n\, A} \\
		                      & = \frac{\sqrt{2}}{A\sqrt{n}}
	\end{align*}
	Using a different method, we will prove that $2^{-2n} \binom{2n}{n} \sim \frac{1}{\sqrt{\pi n}}$, which then forces $A = \sqrt{2\pi}$. Consider
	\[ I_n = \int_0^{\frac{\pi}{2}} (\cos \theta)^n \, \dd \theta;\quad n \geq 0 \]
	So $I_0 = \frac{\pi}{2}$ and $I_1 = 1$. By integrating by parts,
	\[ I_n = \frac{n-1}{n}I_{n-2} \]
	Therefore,
	\[ I_{2n} = \frac{2n-1}{2n}I_{2n-2} = \frac{(2n-1)(2n-3)\dots(3)(1)}{(2n)(2n-2)\dots(2)}I_0 \]
	Multiplying the numerator and denominator by the denominator, we have
	\[ I_{2n} = \frac{(2n)!}{(n! \cdot 2^n)^2} \cdot \frac{\pi}{2} = 2^{-2n} \frac{2n}{n} \cdot \frac{\pi}{2} \]
	In the same way, we can deduce that
	\[ I_{2n+1} = \frac{(2n)(2n-2)\dots(2)}{(2n+1)(2n-1)\dots(3)(1)}I_1 = \frac{1}{2n+1} \left( 2^{-2n} \binom{2n}{n} \right)^{-1} \]
	From $I_n = \frac{n-1}{n}I_{n-2}$, we get that
	\[ \frac{I_n}{I_{n-2}} \to 1 \]
	as $n \to \infty$. We now want to show that $\frac{I_{2n}}{I_{2n+1}} \to 1$. We see from the definition of $I_n$ that $I$ is a decreasing function of $n$. Therefore,
	\[ \frac{I_{2n}}{I_{2n+1}} \leq \frac{I_{2n-1}}{I_{2n+1}} \to 1 \]
	and also
	\[ \frac{I_{2n}}{I_{2n+1}} \geq \frac{I_{2n}}{I_{2n-2}} \to 1 \]
	So
	\[ \frac{I_{2n}}{I_{2n+1}} \to 1 \]
	which means that
	\[ \frac{2^{-2n} \binom{2n}{n} \frac{\pi}{2}}{\left( 2^{-2n} \binom{2n}{n} \right)^{-1} \frac{1}{2n+1}} \to 1 \implies \left( 2^{-2n} \binom{2n}{n} \right)^2 \frac{\pi}{2} (2n+1) \to 1 \]
	Therefore,
	\[ \left( 2^{-2n} \binom{2n}{n} \right)^2 \sim \frac{2}{\pi (2n+1)} \sim \frac{1}{\pi n} \]
	Finally,
	\[ A = \sqrt{2 \pi} \]
	completes the proof.
\end{proof}

\subsection{Countable Subadditivity}
Let $(\Omega, \mathcal F, \mathbb P)$ be a probability space, and let $(A_n)_{n \geq 1}$ be a (not necessarily disjoint) sequence of events in $\mathcal F$. Then
\[ \prob{\bigcup_{n=1}^\infty A_n} \leq \sum_{n=1}^\infty \prob{A_n} \]
\begin{proof}
	Let us define a new sequence $B_1 = A_1$ and $B_n = A_n \setminus (A_1 \cup A_2 \cup \dots \cup A_{n-1})$. So by construction, the sequence $B_n$ is a disjoint sequence of events in $\mathcal F$. Note further that the union of all $B_n$ is equal to the union of all $A_n$. So
	\[ \prob{\bigcup_{n=1}^\infty A_n} = \prob{\bigcup_{n=1}^\infty B_n} \]
	By the countable additivity axiom,
	\[ \prob{\bigcup_{n=1}^\infty B_n} = \sum_{n=1}^\infty \prob{B_n} \]
	But $B_n \subseteq A_n$. So $\prob{B_n} \leq A_n$. Therefore,
	\[ \prob{\bigcup_{n=1}^\infty A_n} \leq \sum_{n=1}^\infty \prob{A_n} \]
\end{proof}
